Results relating set equality to subset relation; make arguments implicit.

set_pairs/src/pairs.lean
@@ -1,5 +1,3 @@
-open set
-
 universe u
 
 section
@@ -7,7 +5,7 @@ section
   parameters (α : Type u) (x y : α)
 
   theorem mem_insert
-    (s : set α) : set.mem x (set.insert x s)
+    {s : set α} : set.mem x (set.insert x s)
   := 
     begin
       -- change (set.mem x ({ a | a = x ∨ a ∈ s})),
@@ -20,7 +18,7 @@ section
     end
   -- an alternative (more natural/readable?) proof of mem_insert
   example
-    (s : set α) : set.mem x (set.insert x s)
+    {s : set α} : set.mem x (set.insert x s)
   :=
     begin
       have : x = x, by trivial, -- specifically, by refl
@@ -42,7 +40,12 @@ section
       -- Lean automatically translates the notation x ∈ { x }
       apply mem_insert,
       done
-    end    
+    end
+  -- So, it is just an application of mem_insert
+  example :
+    x ∈ ({ x } : set α)
+  :=
+    by apply mem_insert
   -- Forward proof of singleton_set_mem
   example :
     x ∈ ({ x } : set α)
@@ -52,13 +55,9 @@ section
       show set.mem x ({ x }), from this,
       done
     end
-  example :
-    x ∈ ({ x } : set α)
-  :=
-    by apply mem_insert
 
   theorem set_swap
-    (s : set α) (x y : α) 
+    {s : set α} {x y : α}
       : set.insert x (set.insert y s) = set.insert y (set.insert x s)
   :=
     calc
@@ -66,7 +65,7 @@ section
         : by {congr, funext, from propext or.left_comm}
   -- Trying to do a more explicit calculational proof
   example
-    (s : set α) (x y : α) 
+    {s : set α} {x y : α}
       : set.insert x (set.insert y s) = set.insert y (set.insert x s)
   :=
       calc
@@ -89,7 +88,7 @@ section
           --         : by rw set.insert
   -- 'Explicit' proof of set_swap
   example
-    (s : set α) (x y : α)
+    {s : set α} {x y : α}
       : set.insert x (set.insert y s) = set.insert y (set.insert x s)
   :=
     begin
@@ -116,12 +115,132 @@ section
       done
     end
 
-  -- The set notation { x₁, ..., xₙ } is short-hand for fold_left set.insert ∅ [x₁, ..., xₙ].
+  -- The set notation { x₁, ..., xₙ } is short-hand for
+  --   fold_left set.insert ∅ [x₁, ..., xₙ]
   -- So, {x, y} = fold_left set.insert ∅ [x, y] = set.insert y (set.insert x ∅)
   example :
     ({x, y} : set α) = set.insert x {y}
   :=
     by apply set_swap
+
+  theorem set_eq_iff_subsets
+    {s₁ s₂ : set α} : s₁ = s₂ ↔ s₁ ⊆ s₂ ∧ s₂ ⊆ s₁
+  :=
+    begin
+      split, -- split bi-implication into individual implications
+
+      -- show left-to-right
+      show s₁ = s₂ → s₁ ⊆ s₂ ∧ s₂ ⊆ s₁, by {
+        assume : s₁ = s₂,
+        split, -- show the two conjuncts individually
+
+        show s₁ ⊆ s₂,
+        suffices : ∀ x, x ∈ s₁ → x ∈ s₂, from this, by {
+          intros,
+          show x ∈ s₂, from eq.subst ‹s₁ = s₂› ‹x ∈ s₁›,
+        },
+
+        show s₂ ⊆ s₁,
+        suffices : ∀ x, x ∈ s₂ → x ∈ s₁, from this, by {
+          intros,
+          show x ∈ s₁, from eq.subst (eq.symm ‹s₁ = s₂›) ‹x ∈ s₂›,
+        },
+
+        done
+      },
+
+      -- show right-to-left
+      show s₁ ⊆ s₂ ∧ s₂ ⊆ s₁ → s₁ = s₂, by {
+        assume : s₁ ⊆ s₂ ∧ s₂ ⊆ s₁,
+        have : s₁ ⊆ s₂, from and.left ‹s₁ ⊆ s₂ ∧ s₂ ⊆ s₁›,
+        have : s₂ ⊆ s₁, from and.right ‹s₁ ⊆ s₂ ∧ s₂ ⊆ s₁›,
+
+        have : ∀ x, x ∈ s₁ ↔ x ∈ s₂, by {
+          assume x,
+          split,
+          show x ∈ s₁ → x ∈ s₂,
+            by {assume : x ∈ s₁, show x ∈ s₂, from ‹s₁ ⊆ s₂› this},
+          show x ∈ s₂ → x ∈ s₁,
+            by {assume : x ∈ s₂, show x ∈ s₁, from ‹s₂ ⊆ s₁› this},
+          done
+        },
+
+        show s₁ = s₂,
+        suffices : ∀ (x : α), (x ∈ s₁) = (x ∈ s₂),
+          from funext this,
+        by {
+          assume x,
+          have : x ∈ s₁ ↔ x ∈ s₂, from ‹∀ x, x ∈ s₁ ↔ x ∈ s₂› x,
+          show (x ∈ s₁) = (x ∈ s₂), from propext this,
+          done
+        },
+         
+        done
+      },
+
+      -- and we are done
+      done
+    end
+
+  lemma set_eq_imp_subset_left
+    {s₁ s₂ : set α} : s₁ = s₂ → s₁ ⊆ s₂
+  := 
+    λ eq, and.left (iff.elim_left (set_eq_iff_subsets) eq)
+  -- Explicit proof
+  example
+    {s₁ s₂ : set α} : s₁ = s₂ → s₁ ⊆ s₂
+  := 
+    begin
+      intros,
+      have : s₁ = s₂ ↔ s₁ ⊆ s₂ ∧ s₂ ⊆ s₁, from set_eq_iff_subsets,
+      have : s₁ = s₂ → s₁ ⊆ s₂ ∧ s₂ ⊆ s₁, from iff.elim_left this,
+      have : s₁ ⊆ s₂ ∧ s₂ ⊆ s₁, from this ‹s₁ = s₂›,
+      show s₁ ⊆ s₂, from and.elim_left this,
+      done
+    end
+
+  lemma set_eq_imp_subset_right
+    {s₁ s₂ : set α} : s₁ = s₂ → s₂ ⊆ s₁
+  := 
+    λ eq, and.right (iff.elim_left (set_eq_iff_subsets) eq)
+  -- Explicit proof
+  example
+    {s₁ s₂ : set α} : s₁ = s₂ → s₂ ⊆ s₁
+  := 
+    begin
+      intros,
+      have : s₁ = s₂ ↔ s₁ ⊆ s₂ ∧ s₂ ⊆ s₁, from set_eq_iff_subsets,
+      have : s₁ = s₂ → s₁ ⊆ s₂ ∧ s₂ ⊆ s₁, from iff.elim_left this,
+      have : s₁ ⊆ s₂ ∧ s₂ ⊆ s₁, from this ‹s₁ = s₂›,
+      show s₂ ⊆ s₁, from and.elim_right this,
+      done
+    end
+
+  -- s₁ ⊆ s₂ is notation for set.subset s₁ s₂, which is definitionally equal to
+  --   ∀ ⦃x⦄, x ∈ s₁ → x ∈ s₂
+  -- so we can directly derive (a witness for) x ∈ s₂ by passing (a witness for)
+  -- x ∈ s₁ to (a witness for) s₁ ⊆ s₂, with Lean automatically instantiating
+  -- the universal quantifier
+  example
+    (s₁ s₂ : set α) (x : α) : s₁ ⊆ s₂ → x ∈ s₁ → x ∈ s₂
+  :=
+    begin
+      intros,
+      show x ∈ s₂, from ‹s₁ ⊆ s₂› ‹x ∈ s₁›,
+      done
+    end
+  -- We can make the definition of ⊆ and the instantiation of the universal
+  -- quantifier explicit.
+  example
+    (s₁ s₂ : set α) (x : α) : s₁ ⊆ s₂ → x ∈ s₁ → x ∈ s₂
+  :=
+    begin
+      assume : s₁ ⊆ s₂, assume : x ∈ s₁,
+      have : ∀ y, y ∈ s₁ → y ∈ s₂, from ‹s₁ ⊆ s₂›,
+      have : x ∈ s₁ → x ∈ s₂, from this x,
+      show x ∈ s₂, from this ‹x ∈ s₁›,
+      done
+    end
 
 end
 
@@ -129,17 +248,17 @@ section
 
   parameters (α : Type u) (a₁ a₂ : α) (b₁ b₂ : α)
 
-  def A := ({{a₁}, {a₁, a₂}} : set (set α))
-  def B := ({{b₁}, {b₁,b₂}} : set (set α))
+  def pair (x y : α) : set (set α) := {{x}, {x, y}}
 
-  #check ({a₁, a₂} : set α)
+  def A := pair a₁ a₂
+  def B := pair b₁ b₂
 
-  example :
+  theorem adequacy :
     A = B → a₁ = b₁ ∧ a₂ = b₂
   :=
     begin
-      intro hyp,
-      have : A = {{a₁}, {a₁, a₂}}, by rw A,
+      intro,
+      have : A = {{a₁}, {a₁, a₂}}, by rw [A, pair],
       have : A = set.insert {a₁, a₂} {{a₁}}, by {rw set.insert, from this},
       -- { s | s = {a₁} ∨ s ∈ {{a₁, a₂}}}, by {rw set.insert, from this}
       -- assume : ({{a₁}, {a₁, a₂}} : set (set α)) = {{b₁},{b₁,b₂}},
